Weidenbach_Book/Watched_Literals_List_Restart.thy
@@ -1,5 +1,6 @@
 theory Watched_Literals_List_Restart
-  imports Watched_Literals_List Watched_Literals_Algorithm_Restart Array_UInt
+  imports Watched_Literals.Watched_Literals_List Watched_Literals_Algorithm_Restart
+     Watched_Literals.Array_UInt
 begin
 
 text \<open>
